spec/abstract/Exceptions_A.thy
@@ -57,16 +57,10 @@ definition
 where without_preemption_def[simp]:
  "without_preemption \<equiv> liftE"
 
-text \<open>Allow preemption at this point.\<close>
-definition
-  preemption_point :: "(unit,'z::state_ext) p_monad" where
- "preemption_point \<equiv> doE liftE $ do_extended_op update_work_units;
-                         OR_choiceE (work_units_limit_reached)
-                           (doE liftE $ do_extended_op reset_work_units;
-                                irq_opt \<leftarrow> liftE $ do_machine_op (getActiveIRQ True);
-                                case_option (returnOk ()) (K (throwError $ ())) irq_opt
-                           odE) (returnOk ())
-                     odE"
+text \<open>for MCS, the function preemption\_point is defined in InvocationFuns\_A.thy which imports Ipc\_R.
+This is because of the dependency on update\_time\_stamp and check\_budget. Some invocation functions
+that call preemption\_point, namely, invoke\_untyped, invoke\_cnode, and invoke\_tcb, are also
+defined in InvocationFuns\_A.thy\<close>
 
 text \<open>Lift one kind of exception monad into another by converting the error
 into various other kinds of error or return value.\<close>
