spec/abstract/InvocationFuns_A.thy
@@ -1,0 +1,379 @@
+(*
+ * Copyright 2014, General Dynamics C4 Systems
+ *
+ * SPDX-License-Identifier: GPL-2.0-only
+ *)
+
+(*
+Monad instantiations, handling of faults, errors, and interrupts.
+*)
+
+chapter "Basic Kernel and Exception Monads"
+
+theory InvocationFuns_A
+imports Ipc_A
+begin
+
+section \<open>Allow preemption at this point.\<close>
+definition
+  preemption_point :: "(unit,'z::state_ext) p_monad" where
+ "preemption_point \<equiv> doE liftE $ do_extended_op update_work_units;
+                         OR_choiceE (work_units_limit_reached)
+                           (doE liftE $ do_extended_op reset_work_units;
+                                irq_opt \<leftarrow> liftE $ do_machine_op (getActiveIRQ True);
+                                case_option (do
+                                               update_time_stamp;
+                                               result \<leftarrow> check_budget;
+                                               if (\<not> result)
+                                               then returnOk ()
+                                               else (throwError $ ())
+                                             od)
+                                            (K (throwError $ ())) irq_opt
+                           odE) (returnOk ())
+                     odE"
+
+
+section \<open>invoke\_untyped\<close>
+
+text \<open>Untyped capabilities note a currently free region. Sometimes this
+region is reset during a Retype operation. This progressively clears the
+underlying memory and also the object level representation, moving the free
+region pointer back to the start of the newly cleared region each time.\<close>
+definition
+  reset_untyped_cap :: "cslot_ptr \<Rightarrow> (unit,'z::state_ext) p_monad"
+where
+  "reset_untyped_cap src_slot = doE
+  cap \<leftarrow> liftE $ get_cap src_slot;
+  sz \<leftarrow> returnOk $ bits_of cap;
+  base \<leftarrow> returnOk $ obj_ref_of cap;
+  if free_index_of cap = 0
+    then returnOk ()
+  else doE
+    liftE $ delete_objects base sz;
+  dev \<leftarrow> returnOk $ is_device_untyped_cap cap;
+
+  if dev \<or> sz < reset_chunk_bits
+      then liftE $ do
+        unless dev $ do_machine_op $ clearMemory base (2 ^ sz);
+        set_cap (UntypedCap dev base sz 0) src_slot
+      od
+    else mapME_x (\<lambda>i. doE
+          liftE $ do_machine_op $ clearMemory (base + (of_nat i << reset_chunk_bits))
+              (2 ^ reset_chunk_bits);
+          liftE $ set_cap (UntypedCap dev base sz
+              (i * 2 ^ reset_chunk_bits)) src_slot;
+          preemption_point
+        odE) (rev [i \<leftarrow> [0 ..< 2 ^ (sz - reset_chunk_bits)].
+            i * 2 ^ reset_chunk_bits < free_index_of cap])
+    odE
+  odE"
+
+text \<open>Untyped capabilities confer authority to the Retype method. This
+clears existing objects from a region, creates new objects of the requested type,
+initialises them and installs new capabilities to them.\<close>
+definition
+  invoke_untyped :: "untyped_invocation \<Rightarrow> (unit,'z::state_ext) p_monad"
+where
+"invoke_untyped ui \<equiv> case ui
+    of Retype src_slot reset base retype_base new_type obj_sz slots is_device \<Rightarrow>
+doE
+  whenE reset $ reset_untyped_cap src_slot;
+  liftE $ do
+
+  cap \<leftarrow> get_cap src_slot;
+
+  \<comment> \<open>Update the untyped cap to track the amount of space used.\<close>
+  total_object_size \<leftarrow> return $ (of_nat (length slots) << (obj_bits_api new_type obj_sz));
+  free_ref \<leftarrow> return $ retype_base + total_object_size;
+  set_cap (UntypedCap is_device base (bits_of cap) (unat (free_ref - base))) src_slot;
+
+  \<comment> \<open>Create new objects.\<close>
+  orefs \<leftarrow> retype_region retype_base (length slots) obj_sz new_type is_device;
+  init_arch_objects new_type retype_base (length slots) obj_sz orefs;
+  mapM_x (create_cap new_type obj_sz src_slot is_device) (zip slots orefs)
+od odE"
+
+
+section \<open>invoke\_cnode\<close>
+
+text \<open>The complete recursive delete operation.\<close>
+function (sequential)
+  rec_del :: "rec_del_call \<Rightarrow> (bool * cap,'z::state_ext) p_monad"
+where
+  "rec_del (CTEDeleteCall slot exposed) s =
+ (doE
+    (success, cleanup_info) \<leftarrow> rec_del (FinaliseSlotCall slot exposed);
+    without_preemption $ when (exposed \<or> success) $ empty_slot slot cleanup_info;
+    returnOk undefined
+  odE) s"
+|
+  "rec_del (FinaliseSlotCall slot exposed) s =
+ (doE
+    cap \<leftarrow> without_preemption $ get_cap slot;
+    if cap = NullCap
+    then returnOk (True, NullCap)
+    else (doE
+      is_final \<leftarrow> without_preemption $ is_final_cap cap;
+      (remainder, cleanup_info) \<leftarrow> without_preemption $ finalise_cap cap is_final;
+      if cap_removeable remainder slot
+      then returnOk (True, cleanup_info)
+      else if cap_cyclic_zombie remainder slot \<and> \<not> exposed
+      then doE
+        without_preemption $ set_cap remainder slot;
+        returnOk (False, NullCap)
+      odE
+      else doE
+        without_preemption $ set_cap remainder slot;
+        rec_del (ReduceZombieCall remainder slot exposed);
+        preemption_point;
+        rec_del (FinaliseSlotCall slot exposed)
+      odE
+    odE)
+  odE) s"
+
+| "rec_del (ReduceZombieCall (Zombie ptr bits (Suc n)) slot False) s =
+ (doE
+    cn \<leftarrow> returnOk $ first_cslot_of (Zombie ptr bits (Suc n));
+    assertE (cn \<noteq> slot);
+    without_preemption $ cap_swap_for_delete cn slot;
+    returnOk undefined
+  odE) s"
+|
+ "rec_del (ReduceZombieCall (Zombie ptr bits (Suc n)) slot True) s =
+ (doE
+    end_slot \<leftarrow> returnOk (ptr, nat_to_cref (zombie_cte_bits bits) n);
+    rec_del (CTEDeleteCall end_slot False);
+    new_cap \<leftarrow> without_preemption $ get_cap slot;
+    if new_cap = Zombie ptr bits (Suc n)
+    then without_preemption $ set_cap (Zombie ptr bits n) slot
+    else assertE (new_cap = NullCap \<or>
+                  is_zombie new_cap \<and> first_cslot_of new_cap = slot
+                   \<and> first_cslot_of (Zombie ptr bits (Suc n)) \<noteq> slot);
+    returnOk undefined
+  odE) s"
+|
+ "rec_del (ReduceZombieCall cap slot exposed) s =
+  fail s"
+  by pat_completeness auto
+
+text \<open>Delete a capability by calling the recursive delete operation.\<close>
+definition
+  cap_delete :: "cslot_ptr \<Rightarrow> (unit, 'z::state_ext) p_monad" where
+ "cap_delete slot \<equiv> doE rec_del (CTEDeleteCall slot True); returnOk () odE"
+
+text \<open>Prepare the capability in a slot for deletion but do not delete it.\<close>
+definition
+  finalise_slot :: "cslot_ptr \<Rightarrow> bool \<Rightarrow> (bool * cap,'z::state_ext) p_monad"
+where
+  "finalise_slot p e \<equiv> rec_del (FinaliseSlotCall p e)"
+
+text \<open>Helper functions for the type of recursive delete calls.\<close>
+primrec
+  exposed_rdcall :: "rec_del_call \<Rightarrow> bool"
+where
+  "exposed_rdcall (CTEDeleteCall slot exposed) = exposed"
+| "exposed_rdcall (FinaliseSlotCall slot exposed) = exposed"
+| "exposed_rdcall (ReduceZombieCall cap slot exposed) = exposed"
+
+primrec
+  isCTEDeleteCall :: "rec_del_call \<Rightarrow> bool"
+where
+  "isCTEDeleteCall (CTEDeleteCall slot exposed) = True"
+| "isCTEDeleteCall (FinaliseSlotCall slot exposed) = False"
+| "isCTEDeleteCall (ReduceZombieCall cap slot exposed) = False"
+
+primrec
+  slot_rdcall :: "rec_del_call \<Rightarrow> cslot_ptr"
+where
+  "slot_rdcall (CTEDeleteCall slot exposed) = slot"
+| "slot_rdcall (FinaliseSlotCall slot exposed) = slot"
+| "slot_rdcall (ReduceZombieCall cap slot exposed) = slot"
+
+text \<open>Revoke the derived capabilities of a given capability, deleting them
+all.\<close>
+
+function cap_revoke :: "cslot_ptr \<Rightarrow> (unit, 'z::state_ext) p_monad"
+where
+"cap_revoke slot s = (doE
+    cap \<leftarrow> without_preemption $ get_cap slot;
+    cdt \<leftarrow> without_preemption $ gets cdt;
+    descendants \<leftarrow> returnOk $ descendants_of slot cdt;
+    whenE (cap \<noteq> NullCap \<and> descendants \<noteq> {}) (doE
+      child \<leftarrow> without_preemption $ select_ext (next_revoke_cap slot) descendants;
+      cap \<leftarrow> without_preemption $ get_cap child;
+      assertE (cap \<noteq> NullCap);
+      cap_delete child;
+      preemption_point;
+      cap_revoke slot
+    odE)
+odE) s"
+by auto
+
+text \<open>Invoking CNode capabilities\<close>
+
+text \<open>The CNode capability confers authority to various methods
+which act on CNodes and the capabilities within them. Copies of
+capabilities may be inserted in empty CNode slots by
+Insert. Capabilities may be moved to empty slots with Move or swapped
+with others in a three way rotate by Rotate. A Reply capability stored
+in a thread's last-caller slot may be saved into a regular CNode slot
+with Save.  The Revoke, Delete and Recycle methods may also be
+invoked on the capabilities stored in the CNode.\<close>
+
+definition
+  invoke_cnode :: "cnode_invocation \<Rightarrow> (unit, 'z::state_ext) p_monad" where
+  "invoke_cnode i \<equiv> case i of
+    RevokeCall dest_slot \<Rightarrow> cap_revoke dest_slot
+  | DeleteCall dest_slot \<Rightarrow> cap_delete dest_slot
+  | InsertCall cap src_slot dest_slot \<Rightarrow>
+       without_preemption $ cap_insert cap src_slot dest_slot
+  | MoveCall cap src_slot dest_slot \<Rightarrow>
+       without_preemption $ cap_move cap src_slot dest_slot
+  | RotateCall cap1 cap2 slot1 slot2 slot3 \<Rightarrow>
+       without_preemption $
+       if slot1 = slot3 then
+         cap_swap cap1 slot1 cap2 slot2
+       else
+         do cap_move cap2 slot2 slot3; cap_move cap1 slot1 slot2 od
+  | CancelBadgedSendsCall (EndpointCap ep b R) \<Rightarrow>
+    without_preemption $ when (b \<noteq> 0) $ cancel_badged_sends ep b
+  | CancelBadgedSendsCall _ \<Rightarrow> fail"
+
+
+
+section \<open>invoke\_tcb\<close>
+
+definition
+  install_tcb_cap :: "obj_ref \<Rightarrow> cslot_ptr \<Rightarrow> nat \<Rightarrow> (cap \<times> cslot_ptr) option \<Rightarrow> (unit, 'z::state_ext) p_monad"
+where
+  "install_tcb_cap target slot n slot_opt \<equiv>
+     case slot_opt of None \<Rightarrow> returnOk ()
+     | Some (new_cap, src_slot) \<Rightarrow> doE
+      cap_delete (target, tcb_cnode_index n);
+      unlessE (new_cap = NullCap) $
+              liftE $ check_cap_at new_cap src_slot
+                    $ check_cap_at (ThreadCap target) slot
+                    $ cap_insert new_cap src_slot (target, tcb_cnode_index n)
+    odE"
+
+definition
+  install_tcb_frame_cap :: "obj_ref \<Rightarrow> cslot_ptr \<Rightarrow> (vspace_ref \<times> (cap \<times> cslot_ptr) option) option \<Rightarrow> (unit, 'z::state_ext) p_monad"
+where
+  "install_tcb_frame_cap target slot buffer \<equiv>
+     case buffer of
+       None \<Rightarrow> returnOk ()
+     | Some (ptr, frame)
+         \<Rightarrow> doE
+              cap_delete (target, tcb_cnode_index 2);
+              liftE $ thread_set (\<lambda>t. t \<lparr> tcb_ipc_buffer := ptr \<rparr>) target;
+              liftE $ case frame of
+                        None \<Rightarrow> return ()
+                      | Some (new_cap, src_slot)
+                          \<Rightarrow>  check_cap_at new_cap src_slot
+                              $ check_cap_at (ThreadCap target) slot
+                              $ cap_insert new_cap src_slot (target, tcb_cnode_index 2);
+              cur \<leftarrow> liftE $ gets cur_thread;
+              liftE $ when (target = cur) reschedule_required
+            odE"
+
+text \<open>TCB capabilities confer authority to perform seven actions. A thread can
+request to yield its timeslice to another, to suspend or resume another, to
+reconfigure another thread, or to copy register sets into, out of or between
+other threads.\<close>
+fun
+  invoke_tcb :: "tcb_invocation \<Rightarrow> (data list, 'z::state_ext) p_monad"
+where
+  "invoke_tcb (Suspend thread) = liftE (do suspend thread; return [] od)"
+| "invoke_tcb (Resume thread) = liftE (do restart thread; return [] od)"
+
+| "invoke_tcb (ThreadControlCaps target slot fault_handler timeout_handler croot vroot buffer)
+   = doE
+    install_tcb_cap target slot 3 fault_handler;
+    install_tcb_cap target slot 4 timeout_handler;
+    install_tcb_cap target slot 0 croot;
+    install_tcb_cap target slot 1 vroot;
+    install_tcb_frame_cap target slot buffer;
+    returnOk []
+  odE"
+
+| "invoke_tcb (ThreadControlSched target slot fault_handler mcp priority sc)
+   = doE
+    install_tcb_cap target slot 3 fault_handler;
+    liftE $ maybeM (\<lambda>(newmcp, _). set_mcpriority target newmcp) mcp;
+    liftE $ maybeM (\<lambda>(prio, _). set_priority target prio) priority;
+    liftE $ maybeM (\<lambda>scopt. case scopt of
+                              None \<Rightarrow> maybe_sched_context_unbind_tcb target
+                            | Some sc_ptr \<Rightarrow> maybe_sched_context_bind_tcb sc_ptr target) sc;
+    returnOk []
+  odE"
+
+| "invoke_tcb (CopyRegisters dest src suspend_source resume_target transfer_frame transfer_integer transfer_arch) =
+  (liftE $ do
+    when suspend_source $ suspend src;
+    when resume_target $ restart dest;
+    when transfer_frame $ do
+        mapM_x (\<lambda>r. do
+                v \<leftarrow> as_user src $ getRegister r;
+                as_user dest $ setRegister r v
+        od) frame_registers;
+        pc \<leftarrow> as_user dest getRestartPC;
+        as_user dest $ setNextPC pc
+    od;
+    when transfer_integer $
+        mapM_x (\<lambda>r. do
+                v \<leftarrow> as_user src $ getRegister r;
+                as_user dest $ setRegister r v
+        od) gpRegisters;
+    cur \<leftarrow> gets cur_thread;
+    arch_post_modify_registers cur dest;
+    when (dest = cur) reschedule_required;
+    return []
+  od)"
+
+| "invoke_tcb (ReadRegisters src suspend_source n arch) =
+  (liftE $ do
+    when suspend_source $ suspend src;
+    self \<leftarrow> gets cur_thread;
+    regs \<leftarrow> return (take (unat n) $ frame_registers @ gp_registers);
+    as_user src $ mapM getRegister regs
+  od)"
+
+| "invoke_tcb (WriteRegisters dest resume_target values arch) =
+  (liftE $ do
+    self \<leftarrow> gets cur_thread;
+    b \<leftarrow> arch_get_sanitise_register_info dest;
+    as_user dest $ do
+        zipWithM (\<lambda>r v. setRegister r (sanitise_register b r v))
+            (frameRegisters @ gpRegisters) values;
+        pc \<leftarrow> getRestartPC;
+        setNextPC pc
+    od;
+    arch_post_modify_registers self dest;
+    when resume_target $ restart dest;
+    when (dest = self) reschedule_required;
+    return []
+  od)"
+
+| "invoke_tcb (NotificationControl tcb (Some ntfnptr)) =
+  (liftE $ do
+    bind_notification tcb ntfnptr;
+    return []
+  od)"
+
+| "invoke_tcb (NotificationControl tcb None) =
+  (liftE $ do
+    unbind_notification tcb;
+    return []
+  od)"
+
+| "invoke_tcb (SetTLSBase tcb tls_base) =
+  (liftE $ do
+    as_user tcb $ setRegister tlsBaseRegister tls_base;
+    cur \<leftarrow> gets cur_thread;
+    when (tcb = cur) reschedule_required;
+    return []
+  od)"
+
+
+
+end
